{
 "cells": [
  {
   "cell_type": "markdown",
   "metadata": {},
   "source": [
    "## **All You Need To Know About Summation**\n",
    "\n",
    "#### **Summation notation is a compact way of writing the sum of a series of terms. It uses the Greek capital letter sigma (∑) to indicate that you are summing a sequence of numbers defined by a specific formula.**\n",
    "\n",
    "### **Basic Structure:**\n",
    "\n",
    "A typical summation expression looks like this:\n",
    "\n",
    "$$\n",
    "\\sum_{i=a}^{b} f(i)\n",
    "$$\n",
    "\n",
    "- **$\\sum$**: This is the summation symbol.\n",
    "- **$i$**: This is the index of summation; it represents each term's position.\n",
    "- **$a$**: The lower limit; the summation starts with $i = a$.\n",
    "- **$b$**: The upper limit; the summation continues until $i = b$.\n",
    "- **$f(i)$**: This is the general term (or formula) that depends on $i$.\n",
    "\n",
    "### **Example 1: Simple Sum of Natural Numbers**\n",
    "\n",
    "To sum the first 5 natural numbers, you write:\n",
    "\n",
    "$$\n",
    "\\sum_{i=1}^{5} i\n",
    "$$\n",
    "\n",
    "This means:\n",
    "\n",
    "$$\n",
    "1 + 2 + 3 + 4 + 5 = 15\n",
    "$$\n",
    "\n",
    "### **Example 2: Sum of Squares**\n",
    "\n",
    "Suppose you want to sum the squares of the first 4 numbers:\n",
    "\n",
    "$$\n",
    "\\sum_{i=1}^{4} i^2\n",
    "$$\n",
    "\n",
    "This expands to:\n",
    "\n",
    "$$\n",
    "1^2 + 2^2 + 3^2 + 4^2 = 1 + 4 + 9 + 16 = 30\n",
    "$$\n",
    "\n",
    "---\n",
    "\n",
    "### **Properties of Summations**\n",
    "\n",
    "1. **Linearity:**  \n",
    "   For any constants $c$ and $d$ and functions $f(i)$ and $g(i)$:\n",
    "   $$\n",
    "   \\sum_{i=a}^{b} [c \\cdot f(i) + d \\cdot g(i)] = c \\sum_{i=a}^{b} f(i) + d \\sum_{i=a}^{b} g(i)\n",
    "   $$\n",
    "2. **Splitting the Sum:**  \n",
    "   You can split a summation over a range into two parts. For example:\n",
    "   $$\n",
    "   \\sum_{i=1}^{b} f(i) = \\sum_{i=1}^{k} f(i) + \\sum_{i=k+1}^{b} f(i)\n",
    "   $$\n",
    "3. **Changing the Index:**  \n",
    "   Sometimes you may want to change the index of summation. For example, if you let $j = i - 1$, then:\n",
    "   $$\n",
    "   \\sum_{i=1}^{n} f(i) = \\sum_{j=0}^{n-1} f(j+1)\n",
    "   $$\n",
    "\n",
    "---\n",
    "\n",
    "## **Properties With Examples:**\n",
    "\n",
    "### **1. Linearity**\n",
    "\n",
    "**Property:**\n",
    "\n",
    "$$\n",
    "\\sum_{i=a}^{b} [c \\cdot f(i) + d \\cdot g(i)] = c \\sum_{i=a}^{b} f(i) + d \\sum_{i=a}^{b} g(i)\n",
    "$$\n",
    "\n",
    "**Example:**  \n",
    "Suppose $f(i) = i^2$, $g(i) = i$, $c = 2$, $d = -3$, and the summation is over $i = 1$ to $4$. Then:\n",
    "\n",
    "$$\n",
    "\\sum_{i=1}^{4} [2 \\cdot i^2 - 3 \\cdot i]\n",
    "$$\n",
    "\n",
    "Using linearity, we can split this into two separate summations:\n",
    "\n",
    "$$\n",
    "\\sum_{i=1}^{4} [2 \\cdot i^2 - 3 \\cdot i] = 2 \\sum_{i=1}^{4} i^2 - 3 \\sum_{i=1}^{4} i\n",
    "$$\n",
    "\n",
    "Now calculate each term separately:\n",
    "\n",
    "- $\\sum_{i=1}^{4} i^2 = 1^2 + 2^2 + 3^2 + 4^2 = 1 + 4 + 9 + 16 = 30$\n",
    "- $\\sum_{i=1}^{4} i = 1 + 2 + 3 + 4 = 10$\n",
    "\n",
    "Substitute these results back:\n",
    "\n",
    "$$\n",
    "2 \\sum_{i=1}^{4} i^2 - 3 \\sum_{i=1}^{4} i = 2(30) - 3(10) = 60 - 30 = 30\n",
    "$$\n",
    "\n",
    "Thus, the result is:\n",
    "\n",
    "$$\n",
    "\\boxed{30}\n",
    "$$\n",
    "\n",
    "---\n",
    "\n",
    "### **2. Splitting the Sum**\n",
    "\n",
    "**Property:**\n",
    "\n",
    "$$\n",
    "\\sum_{i=1}^{b} f(i) = \\sum_{i=1}^{k} f(i) + \\sum_{i=k+1}^{b} f(i)\n",
    "$$\n",
    "\n",
    "**Example:**  \n",
    "Suppose $f(i) = i^2$, and we want to compute $\\sum_{i=1}^{5} i^2$. Let’s split the summation at $k = 3$:\n",
    "\n",
    "$$\n",
    "\\sum_{i=1}^{5} i^2 = \\sum_{i=1}^{3} i^2 + \\sum_{i=4}^{5} i^2\n",
    "$$\n",
    "\n",
    "Now calculate each part:\n",
    "\n",
    "- $\\sum_{i=1}^{3} i^2 = 1^2 + 2^2 + 3^2 = 1 + 4 + 9 = 14$\n",
    "- $\\sum_{i=4}^{5} i^2 = 4^2 + 5^2 = 16 + 25 = 41$\n",
    "\n",
    "Add the results:\n",
    "\n",
    "$$\n",
    "\\sum_{i=1}^{5} i^2 = 14 + 41 = 55\n",
    "$$\n",
    "\n",
    "Thus, the result is:\n",
    "\n",
    "$$\n",
    "\\boxed{55}\n",
    "$$\n",
    "\n",
    "---\n",
    "\n",
    "### **3. Changing the Index**\n",
    "\n",
    "**Property:**  \n",
    "If you let $j = i - 1$, then:\n",
    "\n",
    "$$\n",
    "\\sum_{i=1}^{n} f(i) = \\sum_{j=0}^{n-1} f(j+1)\n",
    "$$\n",
    "\n",
    "**Example:**  \n",
    "Suppose $f(i) = i^3$, and we want to compute $\\sum_{i=1}^{4} i^3$. Let’s change the index by setting $j = i - 1$, so $i = j + 1$. When $i = 1$, $j = 0$, and when $i = 4$, $j = 3$. The summation becomes:\n",
    "\n",
    "$$\n",
    "\\sum_{i=1}^{4} i^3 = \\sum_{j=0}^{3} (j+1)^3\n",
    "$$\n",
    "\n",
    "Now expand $(j+1)^3$ and compute the summation:\n",
    "\n",
    "$$\n",
    "(j+1)^3 = j^3 + 3j^2 + 3j + 1\n",
    "$$\n",
    "\n",
    "So:\n",
    "\n",
    "$$\n",
    "\\sum_{j=0}^{3} (j+1)^3 = \\sum_{j=0}^{3} j^3 + 3 \\sum_{j=0}^{3} j^2 + 3 \\sum_{j=0}^{3} j + \\sum_{j=0}^{3} 1\n",
    "$$\n",
    "\n",
    "Calculate each term:\n",
    "\n",
    "- $\\sum_{j=0}^{3} j^3 = 0^3 + 1^3 + 2^3 + 3^3 = 0 + 1 + 8 + 27 = 36$\n",
    "- $\\sum_{j=0}^{3} j^2 = 0^2 + 1^2 + 2^2 + 3^2 = 0 + 1 + 4 + 9 = 14$\n",
    "- $\\sum_{j=0}^{3} j = 0 + 1 + 2 + 3 = 6$\n",
    "- $\\sum_{j=0}^{3} 1 = 1 + 1 + 1 + 1 = 4$\n",
    "\n",
    "Substitute these results back:\n",
    "\n",
    "$$\n",
    "\\sum_{j=0}^{3} (j+1)^3 = 36 + 3(14) + 3(6) + 4 = 36 + 42 + 18 + 4 = 100\n",
    "$$\n",
    "\n",
    "Thus, the result is:\n",
    "\n",
    "$$\n",
    "\\boxed{100}\n",
    "$$\n",
    "\n",
    "---\n",
    "\n",
    "### **A Simple Application**\n",
    "\n",
    "Suppose you have the summation:\n",
    "\n",
    "$$\n",
    "S = \\sum_{i=1}^{10} (2i + 3)\n",
    "$$\n",
    "\n",
    "You can compute each term and then add them up:\n",
    "\n",
    "- When $i=1$: $2(1) + 3 = 5$\n",
    "- When $i=2$: $2(2) + 3 = 7$\n",
    "- $\\vdots$\n",
    "- When $i=10$: $2(10) + 3 = 23$\n",
    "\n",
    "So, $S = 5 + 7 + 9 + \\dots + 23$.\n",
    "\n",
    "Alternatively, using properties of summation:\n",
    "\n",
    "$$\n",
    "S = \\sum_{i=1}^{10} (2i + 3) = 2 \\sum_{i=1}^{10} i + 3 \\sum_{i=1}^{10} 1\n",
    "$$\n",
    "\n",
    "We know:\n",
    "\n",
    "$$\n",
    "\\sum_{i=1}^{10} i = \\frac{10(10+1)}{2} = 55 \\quad \\text{and} \\quad \\sum_{i=1}^{10} 1 = 10\n",
    "$$\n",
    "\n",
    "Thus,\n",
    "\n",
    "$$\n",
    "S = 2(55) + 3(10) = 110 + 30 = 140\n",
    "$$\n",
    "\n",
    "### **Summary**\n",
    "\n",
    "- **Summation notation ($\\sum$)** compactly represents the sum of a sequence of terms.\n",
    "- The expression $\\sum_{i=a}^{b} f(i)$ means you sum the values of $f(i)$ as $i$ runs from $a$ to $b$.\n",
    "- Basic properties such as linearity help break down and simplify more complex summations.\n"
   ]
  }
 ],
 "metadata": {
  "language_info": {
   "name": "python"
  }
 },
 "nbformat": 4,
 "nbformat_minor": 2
}
